lib/c/lib_intrinsics.h
@@ -21,8 +21,16 @@
 #define Lib_IntTypes_Intrinsics_add_carry_u64(x1, x2, x3, x4) \
   (Hacl_IntTypes_Intrinsics_add_carry_u64(x1, x2, x3, x4))
 
+
+#define Lib_IntTypes_Intrinsics_add_carry_u64_void(x1, x2, x3, x4) \
+  (Hacl_IntTypes_Intrinsics_add_carry_u64_void(x1, x2, x3, x4))
+
+
 #define Lib_IntTypes_Intrinsics_sub_borrow_u64(x1, x2, x3, x4) \
   (Hacl_IntTypes_Intrinsics_sub_borrow_u64(x1, x2, x3, x4))
+
+#define Lib_IntTypes_Intrinsics_sub_borrow_u64_void(x1, x2, x3, x4) \
+  (Hacl_IntTypes_Intrinsics_sub_borrow_u64_void(x1, x2, x3, x4))
 
 #else
 
@@ -43,6 +51,9 @@
   (__GNUC__ < 7 || (__GNUC__ == 7 && (__GNUC_MINOR__ < 2)))
 
 #define Lib_IntTypes_Intrinsics_sub_borrow_u64(x1, x2, x3, x4) \
+  (_subborrow_u64(x1, x3, x2, (long long unsigned int *) x4))
+
+#define Lib_IntTypes_Intrinsics_sub_borrow_u64_void(x1, x2, x3, x4) \
   (_subborrow_u64(x1, x3, x2, (long long unsigned int *) x4))
 
 #else
