code/fallback/Hacl.IntTypes.Intrinsics.fst
@@ -10,7 +10,7 @@ open Lib.Buffer
 open FStar.Mul
 
 #set-options "--fuel 0 --ifuel 0 --z3rlimit 100"
-
+(* 
 val add_carry_u64: cin:uint64 -> x:uint64 -> y:uint64 -> r:lbuffer uint64 (size 1) ->
   Stack uint64
     (requires fun h -> live h r /\ v cin <= 1)
@@ -47,3 +47,71 @@ let sub_borrow_u64 cin x y result1 =
     logand_mask (logor (gt_mask res x) (logand eqlty cin)) (u64 1) 1;
   result1.(0ul) <- res;
   c1
+
+ *)
+[@CInline]
+val add_carry_u64: cin:uint64 -> x:uint64 -> y:uint64 -> r:lbuffer uint64 (size 1) ->
+  Stack uint64
+    (requires fun h -> live h r /\ v cin <= 1)
+    (ensures  fun h0 c h1 ->
+      modifies1 r h0 h1 /\ v c <= 1 /\
+      (let r = Seq.index (as_seq h1 r) 0 in
+       v r + v c * pow2 64 == v x + v y + v cin))
+
+
+let add_carry_u64 cin x y r = 
+  let x1 = to_u128 x +. to_u128 y +. to_u128 cin in 
+  let x2 = logand x1 (u128 0xffffffffffffffff) in 
+  let x3 = shift_right x1 (size 64) in 
+
+  upd r (size 0) (to_u64 x2);
+  
+  to_u64 x3
+
+
+[@CInline]
+val add_carry_u64_void: cin:uint64 -> x:uint64 -> y:uint64 -> r:lbuffer uint64 (size 1) ->
+  Stack unit
+    (requires fun h -> live h r /\ v cin <= 1)
+    (ensures  fun h0 _ h1 ->
+      modifies1 r h0 h1 /\
+      (let r = Seq.index (as_seq h1 r) 0 in
+       v r  == v x + v y + v cin))
+
+
+let add_carry_u64_void cin x y r = 
+  let x1 = to_u128 x +. to_u128 y +. to_u128 cin in 
+  let x2 = logand x1 (u128 0xffffffffffffffff) in 
+  upd r (size 0) (to_u64 x2)
+
+
+[@CInline]
+val sub_borrow_u64: cin:uint64 -> x:uint64 -> y:uint64 -> r:lbuffer uint64 (size 1) ->
+  Stack uint64
+    (requires fun h -> live h r /\ v cin <= 1)
+    (ensures  fun h0 c h1 ->
+      modifies1 r h0 h1 /\
+      (let r = Seq.index (as_seq h1 r) 0 in
+       v r - v c * pow2 64 == v x - v y - v cin))
+
+let sub_borrow_u64 cin x y r = 
+  let x1 = to_u128 x -. to_u128 y -. to_u128 cin in 
+  let x2 = logand x1 (u128 0xffffffffffffffff) in 
+  let x3 = shift_right x1 (size 64) in 
+
+  upd r (size 0) (to_u64 x2);
+  (u64 0) -. (to_u64 x3)
+
+
+[@CInline]
+val sub_borrow_u64_void: cin:uint64 -> x:uint64 -> y:uint64 -> r:lbuffer uint64 (size 1) ->
+  Stack unit
+    (requires fun h -> live h r /\ v cin <= 1)
+    (ensures  fun h0 _ h1 -> modifies1 r h0 h1 /\
+    (let r = Seq.index (as_seq h1 r) 0 in v r == v x - v y - v cin))
+
+let sub_borrow_u64_void cin x y r = 
+  let x1 = to_u128 x -. to_u128 y -. to_u128 cin in 
+  let x2 = logand x1 (u128 0xffffffffffffffff) in 
+  upd r (size 0) (to_u64 x2)
+    
